src/QL/FOL/Tait/semantics.lean
@@ -1,32 +1,32 @@
-import QL.FOL.Tait.calculus
+import QL.FOL.Tait.calculus logic
 
 universes u v
 
 namespace fol
 open_locale logic_symbol aclogic
-variables {L : language.{u}} {m n : ℕ}
+variables {L : language.{u}} {μ : Type v} {μ₁ : Type*} {μ₂ : Type*} {m n : ℕ} {S : Structure L}
 
 namespace Tait
 
 namespace subformula
 
-variables (S : Structure L) {n} {me : fin m → S} {e : fin n → S}
+variables (S) {n} {Φ : μ → S} {e : fin n → S}
 
-@[simp] def val' (me : fin m → S) : ∀ {n} (e : fin n → S), subformula L m n → Prop
+@[simp] def subval' (Φ : μ → S) : ∀ {n} (e : fin n → S), subformula L μ n → Prop
 | n _ verum              := true
 | n _ falsum             := false
-| n e (relation p v)     := S.pr p (subterm.val S me e ∘ v)
-| n e (neg_relation p v) := ¬S.pr p (subterm.val S me e ∘ v)
-| n e (and p q)          := p.val' e ∧ q.val' e
-| n e (or p q)           := p.val' e ∨ q.val' e
-| n e (fal p)            := ∀ x : S, (p.val' (x *> e))
-| n e (ex p)             := ∃ x : S, (p.val' (x *> e))
+| n e (relation p v)     := S.pr p (λ i, subterm.val S Φ e (v i))
+| n e (neg_relation p v) := ¬S.pr p (λ i, subterm.val S Φ e (v i))
+| n e (and p q)          := p.subval' e ∧ q.subval' e
+| n e (or p q)           := p.subval' e ∨ q.subval' e
+| n e (fal p)            := ∀ x : S, (p.subval' (x *> e))
+| n e (ex p)             := ∃ x : S, (p.subval' (x *> e))
 
-@[simp] lemma val'_neg (p : subformula L m n) : val' S me e (∼p) = ¬val' S me e p :=
-by induction p generalizing me e; simp[mlift, ←verum_eq, ←falsum_eq, ←and_eq, ←or_eq, ←not_eq, ←fal_eq, ←ex_eq, or_iff_not_imp_left, *] at*
+@[simp] lemma subval'_neg (p : subformula L μ n) : subval' S Φ e (∼p) = ¬subval' S Φ e p :=
+by induction p generalizing Φ e; simp[mlift, ←verum_eq, ←falsum_eq, ←and_eq, ←or_eq, ←not_eq, ←fal_eq, ←ex_eq, or_iff_not_imp_left, *] at*
 
-@[irreducible] def val (me : fin m → S) (e : fin n → S) : subformula L m n →ₗ Prop :=
-{ to_fun := val' S me e,
+@[irreducible] def subval (Φ : μ → S) (e : fin n → S) : subformula L μ n →ₗ Prop :=
+{ to_fun := subval' S Φ e,
   map_neg' := λ _, by simp,
   map_imply' := λ _ _, by simp[has_arrow.arrow, imply, or_iff_not_imp_left, not_eq],
   map_and' := λ p q, by unfold has_inf.inf; simp; refl,
@@ -34,112 +34,59 @@ by induction p generalizing me e; simp[mlift, ←verum_eq, ←falsum_eq, ←and_
   map_top' := by refl,
   map_bot' := by refl }
 
-@[simp] lemma val_relation {p} (r : L.pr p) (v) :
-  val S me e (relation r v) ↔ S.pr r (subterm.val S me e ∘ v) :=  by simp[val]; refl
+@[reducible] def val (Φ : μ → S) : formula L μ →ₗ Prop := subformula.subval S Φ fin.nil
 
-@[simp] lemma val_neg_relation {p} (r : L.pr p) (v) :
-  val S me e (neg_relation r v) ↔ ¬S.pr r (subterm.val S me e ∘ v) := by simp[val]; refl
+@[simp] lemma subval_relation {p} {r : L.pr p} {v} :
+  subval S Φ e (relation r v) ↔ S.pr r (subterm.val S Φ e ∘ v) :=  by simp[subval]; refl
 
-@[simp] lemma val_fal (p : subformula L m (n + 1)) :
-  val S me e (∀'p) ↔ ∀ x : S, val S me (x *> e) p := by simp[val]; refl
+@[simp] lemma subval_neg_relation {p} {r : L.pr p} {v} :
+  subval S Φ e (neg_relation r v) ↔ ¬S.pr r (subterm.val S Φ e ∘ v) := by simp[subval]; refl
 
-@[simp] lemma val_ex (p : subformula L m (n + 1)) :
-  val S me e (∃'p) ↔ ∃ x : S, val S me (x *> e) p := by simp[val]; refl
+@[simp] lemma subval_fal {p : subformula L μ (n + 1)} :
+  subval S Φ e (∀'p) ↔ ∀ x : S, subval S Φ (x *> e) p := by simp[subval]; refl
+
+@[simp] lemma subval_ex {p : subformula L μ (n + 1)} :
+  subval S Φ e (∃'p) ↔ ∃ x : S, subval S Φ (x *> e) p := by simp[subval]; refl
+
+variables {μ₁ μ₂}
+
+lemma subval_map {f : μ₁ → μ₂} {Φ : μ₂ → S} {p : subformula L μ₁ n} :
+  subval S Φ e (map f p) ↔ subval S (Φ ∘ f) e p :=
+by induction p using fol.Tait.subformula.ind_on; simp[*, (∘), subterm.val_map]
+
+lemma subval_subst {p : subformula L μ (n + 1)} : ∀ {e} {u : subterm L μ n},
+  subval S Φ e (subst u p) ↔ subval S Φ (e <* subterm.val S Φ e u) p :=
+by apply ind_succ_on p; intros; simp[*, (∘), subterm.val_subst, subterm.val_lift, fin.left_right_concat_assoc]
 
 end subformula
-
-namespace formula
-variables (S : Structure L) {m n} (me : fin m → S)
-
-def val : formula L m →ₗ Prop := subformula.val S me fin.nil  
-
-end formula
-
-def models (S : Structure L) (p : formula L m) : Prop := ∀ e, formula.val S e p
-
-infix (name := Tait.models) ` ⊧ᵀ ` :55 := models
-
-namespace sentence
-variables (S : Structure L) (σ : sentence L)
-
-lemma models_iff : S ⊧ᵀ σ ↔ formula.val S fin.nil σ :=
-by simp[models, fin.nil]
-
-end sentence
-/-
-namespace uniform_subformula
-
-variables (S : Structure L) {n} {me : ℕ → S} {e : fin n → S}
-
-@[simp] def val' (me : ℕ → S) : ∀ {n} (e : fin n → S), uniform_subformula L n → Prop
-| n _ verum              := true
-| n _ falsum             := false
-| n e (relation p v)     := S.pr p (uniform_subterm.val S me e ∘ v)
-| n e (neg_relation p v) := ¬S.pr p (uniform_subterm.val S me e ∘ v)
-| n e (and p q)          := p.val' e ∧ q.val' e
-| n e (or p q)           := p.val' e ∨ q.val' e
-| n e (fal p)            := ∀ x : S, (p.val' (x *> e))
-| n e (ex p)             := ∃ x : S, (p.val' (x *> e))
-
-@[simp] lemma val'_neg (p : uniform_subformula L n) : val' S me e (∼p) = ¬val' S me e p :=
-by simp[←not_eq]; induction p generalizing me e; simp[or_iff_not_imp_left, *]
-
-@[irreducible] def val (me : ℕ → S) (e : fin n → S) : uniform_subformula L n →ₗ Prop :=
-{ to_fun := val' S me e,
-  map_neg' := λ _, by simp,
-  map_imply' := λ _ _, by simp[imply_def, or_iff_not_imp_left, ←or_eq],
-  map_and' := λ p q, by unfold has_inf.inf; simp; refl,
-  map_or' := λ p q, by unfold has_sup.sup; simp; refl,
-  map_top' := by refl,
-  map_bot' := by refl }
-
-@[simp] lemma val_relation {p} (r : L.pr p) (v) :
-  val S me e (relation r v) ↔ S.pr r (uniform_subterm.val S me e ∘ v) :=  by simp[val]; refl
-
-@[simp] lemma val_neg_relation {p} (r : L.pr p) (v) :
-  val S me e (neg_relation r v) ↔ ¬S.pr r (uniform_subterm.val S me e ∘ v) := by simp[val]; refl
-
-@[simp] lemma val_fal (p : uniform_subformula L (n + 1)) :
-  val S me e (∀'p) ↔ ∀ x : S, val S me (x *> e) p := by simp[val]; refl
-
-@[simp] lemma val_ex (p : uniform_subformula L (n + 1)) :
-  val S me e (∃'p) ↔ ∃ x : S, val S me (x *> e) p := by simp[val]; refl
-
-@[simp] lemma val_subst : ∀ {n} {e : fin n → S} (t : uniform_subterm L n) (p : uniform_subformula L (n + 1)),
-  val S me e (subst t p) ↔ val S me (e <* t.val S me e) p
-| n e t verum              := by simp[verum_eq]
-| n e t falsum             := by simp[falsum_eq]
-| n e t (relation r v)     := by simp[(∘)]
-| n e t (neg_relation r v) := by simp[(∘)]
-| n e t (and p q)          := by simp[and_eq, val_subst t p, val_subst t q]
-| n e t (or p q)           := by simp[or_eq, val_subst t p, val_subst t q]
-| n e t (fal p)            := by simp[fal_eq, val_subst t.lift p, fin.left_right_concat_assoc]
-| n e t (ex p)             := by simp[ex_eq, val_subst t.lift p, fin.left_right_concat_assoc]
-using_well_founded {rel_tac := λ _ _, `[exact ⟨_, measure_wf (λ x, x.2.2.2.complexity)⟩]}
-
-end uniform_subformula
-
-namespace uniform_formula
-variables (S : Structure L) {m n} (me : ℕ → S)
-
-def val : uniform_formula L →ₗ Prop := uniform_subformula.val S me fin.nil  
-
-end uniform_formula
-
-def uniform_models (S : Structure L) (p : uniform_formula L) : Prop := ∀ e, uniform_formula.val S e p
-
-infix (name := Tait.uniform_models) ` ⊧ᵀᵤ ` :55 := uniform_models
 
 namespace subformula
-variables (S : Structure L) {n} {me : ℕ → S} {e : fin n → S}
+variables (S) {Φ : μ → S}
 
-lemma val_uniform (p : subformula L m n) : uniform_subformula.val S me e p.uniform ↔ val S (λ i, me i) e p :=
-by { induction p; simp[verum_eq, uniform_subformula.verum_eq, falsum_eq, uniform_subformula.falsum_eq,
-     and_eq, uniform_subformula.and_eq, or_eq, uniform_subformula.or_eq, fal_eq, uniform_subformula.fal_eq,
-     ex_eq, uniform_subformula.ex_eq, (∘), *] }
+notation S` ⊧ᵀ[`:80 e`] `p :50 := val S e p
+
+variables {S} {p q : formula L μ}
+
+@[simp] lemma models_relation {k} {r : L.pr k} {v} :
+  S ⊧ᵀ[Φ] relation r v ↔ S.pr r (λ i, subterm.val S Φ fin.nil (v i)) := by simp[val]
 
 end subformula
--/
+
+def models (S : Structure L) (p : formula L μ) : Prop := ∀ e, S ⊧ᵀ[e] p
+
+instance : logic.semantics (formula L μ) (Structure L) := ⟨models⟩
+
+lemma models_def {S : Structure L} {p : formula L μ} : S ⊧ p ↔ (∀ e, S ⊧ᵀ[e] p) := by refl
+
+lemma sentence_models_def {S : Structure L} {σ : sentence L} : S ⊧ σ ↔ S ⊧ᵀ[fin.nil] σ := by simp[models_def, fin.nil]
+
+--@[simp] lemma models_neg {σ : sentence L} :
+--  S ⊧ ∼σ ↔ ¬S ⊧ σ := by simp[sentence_models_def]
+
+@[simp] lemma models_coe {S : Structure L} {σ : sentence L} {e : μ → S} : S ⊧ᵀ[e] ↑σ ↔ S ⊧ σ :=
+by { simp[subformula.sentence_coe_def, sentence_models_def, subformula.val, subformula.subval_map,
+       show e ∘ fin.nil = fin.nil, by ext x; exact fin.nil x] }
+
 end Tait
 
 end fol
